\documentclass[10pt,a4paper]{article}
\usepackage[latin1]{inputenc}
\usepackage{amsmath}
\usepackage{amsfonts}
\usepackage{amssymb}
\author{Sliven Carranza}
\begin{document}
\begin{center}
         \huge{Hoja de trabajo \#2} \\
        \large{Sliven Carranza Briones 20181393} \\       
\end{center}

\section*{Ejercicio \#1 }
Demostracion de: \\ \\
       $ \forall\ n.\ n^3\geq n^2$ \\ \\
Caso base: \\ \\       
       n=0 \\ \\
        $  n^3\geq n^2$ \\ \\
        $  0^3\geq 0^2$ \\ \\
        $  0\geq 0$ \\ \\
Demostracion Inductiva: \\ \\
n=  n+1 (Sucesor)\\ \\
$ \forall\ n.\ n^3\geq n^2$ \\ \\
$ (n+1)^3\geq (n+1)^2$ \\ \\
$ (n+1)^3 / (n+1)^2  \geq 1 $ \\ \\
$ (n+1)^1  \geq 1 $ \\ \\
$ (n+1) \geq 1 $ \\ \\
$ (n+1)-1 \geq 1 -1 $ \\ \\
$ n \geq 0 $ \\ \\ \\ 

\section*{Ejercicio \#2 } 
Demostracion  inductiva de la desigual\begin{center}
â€¢
\end{center}dad de Bernoulli: \\ \\
        $\forall\ n.\ (1+x)^n\geq nx$ \\ \\
        Caso base : \\ \\
       n=0 \\ \\
       x=0  \\ \\
       $(1+0)^0\geq 0*0$ \\ \\
       $1 \geq 0 $ \\ \\
       
       Demostracion Inductiva: \\ \\
        $(1+x)^n\geq nx+1$ \\ \\
n = n+1\\ \\        
        $(1+x)^{n+1}\geq (n+1)x+1$ \\ \\
         $(1+x)^n*(1+x)^1 \geq (nx+1)*(1+x)$ \\ \\ 
$(1+x)^n*(1+x)^1 \geq nx+nx^2+1+x$ \\ \\
$(1+x)^n*(1+x)^1 \geq (n+1)x+nx^2+ 1$\\ \\
$(1+x)^{n+1} \geq (n+1)x+ 1$\\ \\

\end{document}